Revert "merge subG, invG, sinvG into sinvG."
This reverts commit a78c00b4c61a6f3755e35a038a0b5ca53cf6d7e2.

imp_system/mem/MemA.v
@@ -9,72 +9,64 @@ Canonical Structure valO := leibnizO val.
 Definition frac_valO := prodR fracR (exclR valO).
 Definition _memRA := (mblock -d> Z -d> optionUR frac_valO).
 Definition memRA := authUR _memRA.
-Class memG `{!sinvG Γ Σ α β τ} := {
+Class memGΓ (Γ : HRA) := {
   #[global] mem_inG :: inG memRA Γ;
 }.
-Global Arguments memG Γ Σ α β τ {_}.
 Definition memΓ : HRA := #[memRA].
-Global Instance subG_memΓ `{!sinvG Γ Σ α β τ} : subG memΓ Γ → memG Γ Σ α β τ.
+Global Instance subG_memΓ {Γ: HRA} : subG memΓ Γ → memGΓ Γ.
 Proof. solve_inG. Defined.
 Hint Unfold subG_memΓ mem_inG : GRA_index.
 
-Section Resource.
-  
-  Context `{!sinvG Γ Σ α β τ, !memG Γ Σ α β τ}.
-    
-  (* Initial resources for memory *)
-  Definition mem_init_val (csl : string → bool) genv blk ofs : option Z :=
-    match List.nth_error genv blk with
-    | Some (g, gd) =>
-      match gd↓ with
-      | Some (Gvar gv) => if negb (csl g) && (decide (ofs = 0%Z)) then Some gv else None
-      | _ => None
-      end
-    | None => None
-    end.
+(* Initial resources for memory *)
+Definition mem_init_val (csl : string → bool) genv blk ofs : option Z :=
+  match List.nth_error genv blk with
+  | Some (g, gd) =>
+    match gd↓ with
+    | Some (Gvar gv) => if negb (csl g) && (decide (ofs = 0%Z)) then Some gv else None
+    | _ => None
+    end
+  | None => None
+  end.
 
-  Definition mem_init_auth_r (csl : string → bool) (genv: GEnv.t) : memRA :=
-    ● ((λ blk ofs,
-        match mem_init_val csl genv blk ofs with
-        | Some gv => Some (1%Qp, Excl (Vint gv))
-        | _ => ε
-        end) : _memRA).
+Definition mem_init_auth_r (csl : string → bool) (genv: GEnv.t) : memRA :=
+  ● ((λ blk ofs,
+      match mem_init_val csl genv blk ofs with
+      | Some gv => Some (1%Qp, Excl (Vint gv))
+      | _ => ε
+      end) : _memRA).
 
-  Definition mem_init_frag_r (csl : string → bool) (genv : GEnv.t) : memRA :=
-    ◯ ((λ blk ofs,
-        match mem_init_val csl genv blk ofs with
-        | Some gv => Some (1%Qp, Excl (Vint gv))
-        | _ => ε
-        end) : _memRA).
+Definition mem_init_frag_r (csl : string → bool) (genv : GEnv.t) : memRA :=
+  ◯ ((λ blk ofs,
+      match mem_init_val csl genv blk ofs with
+      | Some gv => Some (1%Qp, Excl (Vint gv))
+      | _ => ε
+      end) : _memRA).
 
-  Definition mem_init_auth csl genv  : iProp Σ :=
-    own base_γ (mem_init_auth_r csl genv).
+Definition mem_init_auth csl genv `{!invG α Σ Γ, !subG Γ Σ, !sinvG Σ Γ α β τ, !memGΓ Γ} : iProp Σ :=
+  own base_γ (mem_init_auth_r csl genv).
 
-  Definition mem_init_frag csl genv : iProp Σ :=
-    own base_γ (mem_init_auth_r csl genv).
+Definition mem_init_frag csl genv `{!invG α Σ Γ, !subG Γ Σ, !sinvG Σ Γ α β τ, !memGΓ Γ} : iProp Σ :=
+  own base_γ (mem_init_auth_r csl genv).
 
-  Definition mem_init csl genv : iProp Σ :=
-    own base_γ (mem_init_auth_r csl genv ⋅ mem_init_frag_r csl genv).
+Definition mem_init csl genv `{!invG α Σ Γ, !subG Γ Σ, !sinvG Σ Γ α β τ, !memGΓ Γ} : iProp Σ :=
+  own base_γ (mem_init_auth_r csl genv ⋅ mem_init_frag_r csl genv).
 
-  Lemma mem_init_valid (csl : string → bool) (genv : GEnv.t) :
-    ✓ (mem_init_auth_r csl genv ⋅ mem_init_frag_r csl genv).
-  Proof using. rewrite /mem_init_auth_r /mem_init_frag_r auth_both_valid_discrete; split; ii; des_ifs. Qed.
+Lemma mem_init_valid (csl : string → bool) (genv : GEnv.t) :
+  ✓ (mem_init_auth_r csl genv ⋅ mem_init_frag_r csl genv).
+Proof. rewrite /mem_init_auth_r /mem_init_frag_r auth_both_valid_discrete; split; ii; des_ifs. Qed.
 
-  Definition ir_memRA csl genv : DRA_mk memRA :=
-    mem_init_auth_r csl genv ⋅ mem_init_frag_r csl genv.
+Definition ir_memRA csl genv : DRA_mk memRA :=
+  mem_init_auth_r csl genv ⋅ mem_init_frag_r csl genv.
+Lemma ir_memRA_valid csl genv : ✓ (ir_memRA csl genv).
+Proof. pose proof (mem_init_valid csl genv). rewrite /ir_memRA //. Qed.
 
-  Lemma ir_memRA_valid csl genv : ✓ (ir_memRA csl genv).
-  Proof using. pose proof (mem_init_valid csl genv). rewrite /ir_memRA //. Qed.
-
-  Definition ir_memΓ csl genv : memΓ :=
-    *[Some (ir_memRA csl genv)].
-
-End Resource.
+Definition ir_memΓ csl genv : memΓ :=
+  *[Some (ir_memRA csl genv)].
 
 Local Arguments Z.of_nat : simpl nomatch.
 
 Section MemRA.
-  Context `{!sinvG Γ Σ α β τ, !memG Γ Σ α β τ}.
+  Context `{!invG α Σ Γ, !subG Γ Σ, !sinvG Σ Γ α β τ, !memGΓ Γ}.
 
   Definition mem_val : Type := Qp * val.
 
@@ -99,7 +91,7 @@ Section MemRA.
   Lemma mem_init_auth_r_valid (csl : string → bool) (genv : GEnv.t) blk ofs v :
     mem_init_val csl genv blk ofs = Some v →
     mem_points_to_singleton_r (blk, ofs) 1 (Vint v) ≼ mem_init_frag_r csl genv.
-  Proof using.
+  Proof.
     intros H. rewrite /mem_init_auth_r /mem_points_to_singleton_r /mem_init_val; ss.
     rewrite /mem_init_frag_r. apply auth_frag_mono.
     match goal with
@@ -131,7 +123,7 @@ Notation "loc ↦ v" := (<own> base_γ (mem_points_to_singleton_r loc 1 v))%SAT 
 Notation "loc |-> vs" := (mem_points_to loc 1 vs) (at level 20).
 
 Module MemA. Section MemA.
-  Context `{!sinvG Γ Σ α β τ, !memG Γ Σ α β τ}.
+  Context `{!invG α Σ Γ, !subG Γ Σ, !sinvG Σ Γ α β τ, !memGΓ Γ}.
 
   Definition scopes := ["Mem"].
 
