apc/APC.v
@@ -73,7 +73,7 @@ Section apc.
 End apc.
 
 Section aux.
-  Context `{!sinvG Γ Σ α β τ}.
+  Context `{!invG α Σ Γ, !subG Γ Σ, !sinvG Σ Γ α β τ}.
 
   Lemma map_fst_map_map_snd_refl {A B C} (f: B → C) (l: list (A * B)):
     map fst (map (map_snd f) l) = map fst l.
