scheduler/SchA.v
@@ -9,7 +9,7 @@ Set Implicit Arguments.
 Local Open Scope Qp.
 
 Section SchRA.
-  Context `{!sinvG Γ Σ α β τ}.
+  Context `{!invG α Σ Γ, !subG Γ Σ, !sinvG Σ Γ α β τ}.
 
   Canonical Structure SynDepO : ofe := leibnizO {n & GTerm.t n}.
 
@@ -20,21 +20,20 @@ Section SchRA.
 
   Definition tidRA : ucmra := nat -d> excl' unit.
 
-  Class schG `{!sinvG Γ Σ α β τ} := {
-      #[local] RA_inG0 :: inG tidRA Γ;
-      #[local] RA_inG :: inG threadsRA Σ;
-    }.
-  Definition schΓ : HRA := #[tidRA].
-  Definition schΣ : GRA := #[threadsRA].
-  Global Instance subG_G : subG schΓ Γ → subG schΣ Σ → schG.
+  Class SchAGΣ (Σ: GRA) := { #[local] RA_inG :: inG threadsRA Σ }.
+  Class SchAGΓ (Γ: HRA) := { #[local] RA_inG0 :: inG tidRA Γ }.
+  Definition SchAΣ : GRA := #[threadsRA].
+  Definition SchAΓ : HRA := #[tidRA].
+  Global Instance subG_GΣ {Σ'} : subG SchAΣ Σ' → SchAGΣ Σ'.
+  Proof using. solve_inG. Defined.
+  Global Instance subG_GΓ {Γ' : HRA} : subG SchAΓ Γ' → SchAGΓ Γ'.
   Proof using. solve_inG. Defined.
 End SchRA.
-Global Arguments schG Γ Σ α β τ {_}.
-Hint Unfold RA_inG RA_inG0 schΣ schΓ : GRA_index.
+Hint Unfold RA_inG RA_inG0 subG_GΣ SchAΣ subG_GΓ SchAΓ : GRA_index.
 
 Module SchAS. Section SchAS.
   Local Existing Instances RA_inG RA_inG0.
-  Context `{!sinvG Γ Σ α β τ, !schG Γ Σ α β τ}.
+  Context `{!invG α Σ Γ, !subG Γ Σ, !sinvG Σ Γ α β τ, !SchAGΣ Σ, !SchAGΓ Γ}.
 
   (** thread **)
   Definition token_pending_r (tid: nat): threadsRA :=
@@ -111,10 +110,10 @@ Module SchAS. Section SchAS.
     tid_admin_r None.
   Lemma ir_tidRA_valid : ✓ (ir_tidRA). intro i; ss. Qed.
 
-  Definition ir_schΓ : schΓ :=
+  Definition ir_SchAΓ : SchAΓ :=
     *[Some ir_tidRA].
 
-  Definition ir_schΣ : schΣ :=
+  Definition ir_SchAΣ : SchAΣ :=
     *[Some ir_threadsRA].
 
   Definition init_threads : iProp Σ := 
@@ -328,7 +327,7 @@ Module SchAS. Section SchAS.
 End SchAS. End SchAS.
 
 Module SchA. Section SchA.
-  Context `{!sinvG Γ Σ α β τ, !schG Γ Σ α β τ}.
+  Context `{!invG α Σ Γ, !subG Γ Σ, !sinvG Σ Γ α β τ, !SchAGΣ Σ, !SchAGΓ Γ}.
 
   Definition scopes := ["Sch"].
   Definition v_internal := "Sch" ↯ "internal".
@@ -393,7 +392,7 @@ End SchA. End SchA.
 Module SchA_link. Section SchA_link.
 
   Definition scopes := ["Tid"].
-  Context `{!sinvG Γ Σ α β τ, !schG Γ Σ α β τ}.
+  Context `{!invG α Σ Γ, !subG Γ Σ, !sinvG Σ Γ α β τ, !SchAGΣ Σ, !SchAGΓ Γ}.
   
   Definition fnsems υ :=
     [(SchHdr.get_tid, (scopes, mk_specbody (SchAS.get_tid_spec υ) fbody_trivial))].
@@ -415,7 +414,8 @@ Module SchA_link. Section SchA_link.
 End SchA_link. End SchA_link.
 
 Section FSPEC.
-  Context `{!sinvG Γ Σ α β τ, !schG Γ Σ α β τ}.
+  Context `{!invG α Σ Γ, !subG Γ Σ, !sinvG Σ Γ α β τ}.
+  Context `{!SchAGΣ Σ, !SchAGΓ Γ}.
 
   Definition sch_fspec υ (fsp : fspec) : fspec :=
     wsim_fspec υ
